theories/program_logic/heap_lang_lifting.v
@@ -11,7 +11,7 @@ Class heapDG Σ := HeapDG {
   heapDG_proph_mapG1 :> proph_mapG proph_id (val*val) Σ;
   heapDG_proph_mapG2 :> proph_mapG proph_id (val*val) Σ;
   heapDG_gen_heapG1 :> gen_heapG loc val Σ;
-  heapDG_gen_heapG2 :> gen_heapG loc val Σ
+  heapDG_gen_heapG2 :> gen_heapG loc val Σ;
 }.
 
 (** irisG instances for both sides *)
